src/rocq/Semantics/Operations/Compare.v
@@ -8,7 +8,7 @@ From Vellvm Require Import
 Section Compare.
   Context {Pa : Params}.
 
-  Definition eval_icmp_h (samesign:bool) (icmp : icmp) (v1 v2 : dvalue) : EOU dvalue.
+  Definition eval_icmp_base (samesign:bool) (icmp : icmp) (v1 v2 : dvalue_base) : EOU dvalue_base.
     refine
       (match v1, v2 with
        | DVALUE_I sz1 i1, DVALUE_I sz2 i2 =>
@@ -17,17 +17,17 @@ Section Compare.
        | DVALUE_Poison t1, DVALUE_Poison t2 => ret (DVALUE_Poison t1)
        | DVALUE_Poison t, _ => if is_DVALUE_IX v2 then ret (DVALUE_Poison t) else raise_error "ill_typed-iop"
        | _, DVALUE_Poison t => if is_DVALUE_IX v1 then ret (DVALUE_Poison t) else raise_error "ill_typed-iop"
-       | DVALUE_Addr a1, DVALUE_Addr a2 =>
+       | DVALUE_Pointer a1, DVALUE_Pointer a2 =>
            let i1 := ptr_to_int a1 in
            let i2 := ptr_to_int a2 in
            eval_int_icmp false icmp i1 i2
-       | _, _ => raise_error ("ill_typed-icmp: " ++ show_dvalue v1 ++ ", " ++ show_dvalue v2)
+       | _, _ => raise_error ("eval_icmp_base: ill_typed-icmp: " ++ show v1 ++ ", " ++ show v2)
        end).
     destruct (Pos.eq_dec sz1 sz2); subst.
     - exact (eval_int_icmp samesign icmp i1 i2).
-    - exact (raise_error ("ill_typed-icmp: " ++ show_dvalue v1 ++ ", " ++ show_dvalue v2)).
+    - exact (raise_error ("eval_icmp_base: ill_typed-icmp: " ++ show v1 ++ ", " ++ show v2)).
   Defined.
-  Arguments eval_icmp_h _ _ _ _ : simpl nomatch.
+  Arguments eval_icmp_base _ _ _ _ : simpl nomatch.
 
   Definition eval_icmp (samesign:bool) (icmp : icmp) (v1 v2 : dvalue) : EOU dvalue :=
     match v1, v2 with
@@ -35,11 +35,12 @@ Section Compare.
         let n := N.length elts1 in
         let m := N.length elts2 in
         if (n =? m)%N  then 
-          val <- vec_loop (eval_icmp_h samesign icmp) (List.combine elts1 elts2) ;;
+          val <- vec_loop (eval_icmp_base samesign icmp) (List.combine elts1 elts2) ;;
           ret (DVALUE_Vector (DTYPE_Vector n (DTYPE_I 1)) val)
         else
           raise_ub "icmp of different-length vectors"
-    | _, _ => eval_icmp_h samesign icmp v1 v2
+    | DVALUE_Base v1, DVALUE_Base v2 => DVALUE_Base <$> (eval_icmp_base samesign icmp v1 v2)
+    | _, _ => raise_error "eval_icmp_base: ill-typed icmp"
     end.
 
   Arguments eval_icmp _ _ _ _ : simpl nomatch.
