src/rocq/Semantics/Operations/Select.v
@@ -8,48 +8,55 @@ From Vellvm Require Import
 Section Select.
   Context {Pa : Params}.
 
-  Definition eval_select
-    (cnd : dvalue) (v1 v2 : dvalue) : EOU dvalue
-    := match cnd with
-       | DVALUE_Poison t =>
-           (* TODO: Should be the type of the result of the select... *)
-           ret (DVALUE_Poison t)
-       | DVALUE_I 1 i =>
-           if (@Integers.unsigned 1 i =? 1)%Z
-           then ret v1
-           else ret v2
-       | DVALUE_Vector _ conds =>
-           let fix loop conds xs ys : EOU (list dvalue) :=
-             match conds, xs, ys with
-             | [], [], [] => ret []
-             | (c::conds), (x::xs), (y::ys) =>
-                 selected <- match c with
-                            | DVALUE_Poison t =>
-                                (* TODO: Should be the type of the result of the select... *)
-                                ret (DVALUE_Poison t)
-                            | DVALUE_I 1 i =>
-                                if (@Integers.unsigned 1 i =? 1)%Z
-                                then ret x
-                                else ret y
-                            | _ => raise_error "eval_select: ill-typed select, condition in vector was not poison or i1."
-                            end;;
-                 rest <- loop conds xs ys;;
-                 ret (selected :: rest)
-             | _, _, _ => raise_error "eval_select: ill-typed vector select, length mismatch."
-             end in
-           match v1, v2 with
-           | DVALUE_Poison t, _ =>
-               (* TODO: Should we make sure t is a vector type...? *)
-               ret (DVALUE_Poison t)
-           | DVALUE_Vector _ _, DVALUE_Poison t =>
-               (* TODO: Should we make sure t is a vector type...? *)
-               ret (DVALUE_Poison t)
-           | DVALUE_Vector t xs, DVALUE_Vector _ ys =>
-               selected <- loop conds xs ys;;
-               ret (DVALUE_Vector t selected)
-           | _, _ => raise_error "eval_select: ill-typed vector select, non-vector arguments"
-           end
-       | _ => raise_error "eval_select: ill-typed select."
-       end.
+  Definition eval_select_base (cnd : dvalue_base) (v1 v2 : dvalue_base) : EOU dvalue_base :=
+    match cnd with
+    | DVALUE_Poison (DTYPE_Base (DTYPE_I 1)) =>
+        (* picks the "type" of v1 *)
+        ret (DVALUE_Poison (dtyp_of_dvalue_base v1))
+    | DVALUE_I 1 i =>
+        if (@Integers.unsigned 1 i =? 1)%Z
+        then ret v1
+        else ret v2
+    | _ => raise_error "eval_select_base: ill-typed select."
+    end.
+    
+  Definition eval_select_base_dvalue (cnd : dvalue_base) (v1 v2 : dvalue) : EOU dvalue :=
+    match cnd with
+    | DVALUE_Poison (DTYPE_Base (DTYPE_I 1)) =>
+        (* picks the "type" of v1 *)
+        (fun x => DVALUE_Base (DVALUE_Poison x)) <$> (dtyp_of_dvalue v1)
+    | DVALUE_I 1 i =>
+        if (@Integers.unsigned 1 i =? 1)%Z
+        then ret v1
+        else ret v2
+    | _ => raise_error "eval_select_base_dvalue: ill-typed select."
+    end.
+
+
+
+  Definition eval_select (cnd : dvalue) (v1 v2 : dvalue) : EOU dvalue :=
+    match cnd with
+    | DVALUE_Base cnd' => eval_select_base_dvalue cnd' v1 v2
+    | DVALUE_Vector _ conds =>
+        match v1, v2 with
+        | DVALUE_Vector t elts1, DVALUE_Vector _ elts2 =>
+            (DVALUE_Vector t) <$>
+              (vec_loop (fun c => fun '(v1, v2) => eval_select_base c v1 v2)
+                 (List.combine conds (List.combine elts1 elts2)))
+        | DVALUE_Base (DVALUE_Poison (DTYPE_Vector sz t)), DVALUE_Vector _ ys =>
+            (DVALUE_Vector (DTYPE_Vector sz t)) <$>
+              (vec_loop (fun c => fun '(v1, v2) => eval_select_base c v1 v2)
+                 (List.combine conds (List.combine (repeat (DVALUE_Poison (DTYPE_Base t)) (N.to_nat sz)) ys)))
+        | DVALUE_Vector _ xs, DVALUE_Base (DVALUE_Poison (DTYPE_Vector sz t)) =>
+            (DVALUE_Vector (DTYPE_Vector sz t)) <$>
+              (vec_loop (fun c => fun '(v1, v2) => eval_select_base c v1 v2)
+                 (List.combine conds (List.combine xs (repeat (DVALUE_Poison (DTYPE_Base t)) (N.to_nat sz)))))
+        | DVALUE_Base (DVALUE_Poison (DTYPE_Vector sz t)), DVALUE_Base (DVALUE_Poison (DTYPE_Vector _ _)) =>
+        (* TODO: could check the sizes to see if this is UB *)
+            ret (DVALUE_Base (DVALUE_Poison (DTYPE_Vector sz t)))
+        | _, _ => raise_error "eval_select: ill-typed vector select, non-vector arguments"
+        end
+    | _ => raise_error "eval_select: ill-typed select."
+    end.
 
 End Select.
